compose/Mod.v
@@ -42,7 +42,8 @@ Module Mod.
     get_modsem_projected_sk: forall
       skenv
       ,
-        SkEnv.project skenv data.(get_sk).(defs) = data.(get_modsem skenv).(ModSem.skenv)
+        (* SkEnv.project skenv data.(get_sk).(defs) = data.(get_modsem skenv).(ModSem.skenv) *)
+        <<PROJECTED: SkEnv.project_spec skenv data.(get_sk).(defs) data.(get_modsem skenv).(ModSem.skenv)>>
     ;
     (* TODO: What is the exact spec we need here? *)
     (* get_modsem_sk_skenv_iso: forall *)
